refactor code. remove axiom. beautify code extraction.

UniversalSearch.v
@@ -1,142 +1,99 @@
-Require Export List Program CoqCore.Tactic Omega ClassicalFacts.
+Require Export Omega ClassicalFacts CoqCore.Tactic CoqCore.MoreFunction CoqCore.MoreList Recdef.
 Set Implicit Arguments.
-Axiom PE : prop_extensionality.
-Variable T : Type.
-Variable P : T -> Prop.
-Variable Dec : forall t, { P t } + { ~P t }.
-Variable Machine : Type.
-Variable Step : Machine -> Machine + T.
-Fixpoint iterate { T } n F (x : T) :=
-  match n with
-  | 0 => x
-  | S n' => iterate n' F (F x)
-  end.
-Definition f_iterate T n f : forall x : T, iterate (S n) f x = f (iterate n f x).
-  induction n; simpl in *; trivial.
-Qed.
-Definition StepN n m : Machine + T := 
-  iterate n (fun x => match x with inl m' => Step m' | _ => x end) (inl m).
-Definition StepNS n m M : 
-  StepN n m = inl M -> StepN (S n) m = Step M.
-  unfold StepN; rewrite f_iterate.
-  intros H; rewrite H; trivial.
-Qed.
-Variable AllMachine : nat -> Machine.
-Definition AMSN n m := StepN n (AllMachine m).
-Definition HasSolution n m := exists t, inr t = AMSN n m /\ P t.
-Variable SolutionExists : exists n m, HasSolution n m.
-Definition SmallestSolution n m : Prop := 
-  HasSolution n m /\ forall l r, HasSolution l r -> m + n <= l + r.
-Variable SmallestSolutionExists : exists n m, SmallestSolution n m.
-Fixpoint split_sum L R (l : list (L + R)) : list L * list R :=
-  match l with
-  | [] => ([],[])
-  | inl h :: t => let (l', r') := split_sum t in (h :: l', r')
-  | inr h :: t => let (l', r') := split_sum t in (l', h :: r')
-  end.
+Section UniversalSearch.
+  Variable T : Type.
+  Variable P : T -> Prop.
+  Variable Dec : forall t, { P t } + { ~P t }.
+  Variable Machine : Type.
+  Variable Step : Machine -> Machine + T.
+  Definition StepN n m : Machine + T := 
+    iterate n (fun x => match x with inl m' => Step m' | _ => x end) (inl m).
+  Definition StepNS n m M : 
+    StepN n m = inl M -> StepN (S n) m = Step M.
+    unfold StepN; rewrite f_iterate.
+    intros H; rewrite H; trivial.
+  Qed.
+  Variable AllMachine : nat -> Machine.
+  Definition AMSN n m := StepN n (AllMachine m).
+  Definition IsSolution n m := exists t, inr t = AMSN n m /\ P t.
+  Variable HasSolution : exists n m, IsSolution n m.
 
-Definition Exists_dec_cons (A : Type) (P : A -> Prop) (l : list A) :
-  (forall x : A, {P x} + {~ P x}) -> {x | P x /\ In x l} + {~Exists P l}.
-  induction l; intuition idtac.
-  right; intros; inversion H.
-  destruct a0; intuition eauto with *.
-  destruct (X a); [intuition eauto with *|].
-  right; intros; inversion H; eauto.
-Defined.
-Definition AMSNSL l r m : 
-  AMSN (S l) r = inl m -> exists m', AMSN l r = inl m' /\ Step m' = inl m.
-  intros; unfold AMSN in *.
-  revert m H; generalize (AllMachine r); clear r.
-  induction l; intros; unfold StepN in *.
-  simpl in *; eauto.
-  rewrite !f_iterate in *.
-  repeat match_destruct; try congruence.
-  specialize (IHl m m2); rewrite !f_iterate, !H0 in *; ii.
-  destruct H2; ii.
-  invcs H3; eauto.
-Qed.
-Definition AMSNSR l r t : 
-  AMSN (S l) r = inr t -> 
-  AMSN l r = inr t \/ exists m', AMSN l r = inl m' /\ Step m' = inr t.
-  intros; unfold AMSN in *; unfold StepN in *; rewrite !f_iterate in *.
-  repeat match_destruct; try congruence; eauto.
-Qed.
-Search(well_founded).
-Program Fixpoint UniversalSearchAux 
-  (n : {n | forall l r, SmallestSolution l r -> n <= l + r})
-  (m : list Machine) 
-  {wf (fun l r => r < l /\ forall n m, SmallestSolution n m -> l <= n + m) n } : 
-  (forall l r, 
-    l + r = n -> 
-    match AMSN l r with
-    | inl M => In M m
-    | inr t => ~P t
-    end) ->
-  { t | P t } :=
-  fun H =>
-  let map_step := split_sum (map Step m) in
-  match Exists_dec_cons P (snd map_step) Dec with
-  | inleft X => X
-  | inright X => @UniversalSearchAux (S n) (AllMachine (S n) :: (fst map_step)) _ _
-  end.
-Obligation Tactic := repeat (ii; subst).
-Definition split_sum_In_fst L R (l : list (L + R)) t : 
-  In (inl t) l <-> In t (fst (split_sum l)).
-  split; induction l; intros; simpl in *; trivial; ii; subst; simpl in *;
-  destruct split_sum eqn:?; simpl in *; ii.
-  destruct a; simpl in *; ii; subst; ii.
-Defined.
-Definition split_sum_In_snd L R (l : list (L + R)) t : 
-  In (inr t) l <-> In t (snd (split_sum l)).
-  split; induction l; intros; simpl in *; trivial; ii; subst; simpl in *;
-  destruct split_sum eqn:?; simpl in *; ii.
-  destruct a; simpl in *; ii; subst; ii.
-Defined.
-Next Obligation.
-  destruct n; simpl in *.
-  specialize (l0 l r); ii.
-  destruct (Nat.eq_dec (l + r) x); subst; try omega.
-  exfalso; specialize(H l r eq_refl); unfold HasSolution in *.
-  unfold SmallestSolution, HasSolution in *; ii.
-  destruct H2; match_destruct; ii; congruence.
-Defined.
+  Definition AMSNSL l r m : 
+    AMSN (S l) r = inl m -> exists m', AMSN l r = inl m' /\ Step m' = inl m.
+    intros; unfold AMSN in *.
+    revert m H; generalize (AllMachine r); clear r.
+    induction l; intros; unfold StepN in *.
+    simpl in *; eauto.
+    rewrite !f_iterate in *.
+    repeat match_destruct; try congruence.
+    specialize (IHl m m2); rewrite !f_iterate, !H0 in *; ii.
+    destruct H2; ii.
+    invcs H3; eauto.
+  Qed.
+  Definition AMSNSR l r t : 
+    AMSN (S l) r = inr t -> 
+    AMSN l r = inr t \/ exists m', AMSN l r = inl m' /\ Step m' = inr t.
+    intros; unfold AMSN in *; unfold StepN in *; rewrite !f_iterate in *.
+    repeat match_destruct; try congruence; eauto.
+  Qed.
+  Definition R l r := l = S r /\ forall n m, IsSolution n m -> l <= n + m.
+  Definition WFR : well_founded R.
+    destruct HasSolution as [? []]; clear HasSolution.
+    unfold well_founded; intros.
+    assert({n | n = x + x0 - a}) by eauto; destruct H0.
+    revert H e; revert a.
+    induction x1; intros.
+    destruct(lt_dec (x + x0) a).
+    constructor; intros; exfalso; unfold R in *; ii; subst.
+    specialize(H2 _ _ H); omega.
+    assert(a = x + x0) by omega; subst.
+    constructor; intros; exfalso; unfold R in *; ii; subst.
+    specialize(H2 _ _ H); omega.
+    constructor; intros; unfold R in *; ii; subst.
+    apply IHx1; auto; omega.
+  Qed.
+  Definition UniversalSearchAux (n : nat) (m : list Machine) : 
+    (forall l r, 
+      l + r = n -> 
+      match AMSN l r with
+      | inl M => In M m
+      | inr t => ~P t
+      end) ->
+    (forall l r, IsSolution l r -> n <= l + r) ->
+    { t | P t }.
+    revert m; refine (Wf.Fix WFR (fun _ => _) _ n).
+    intros; unfold R in *.
+    pose (map_step := split_sum (map Step m)).
+    destruct (Exists_dec_cons P (snd map_step) Dec) as [[]|]; ii; eauto.
+    eapply X; ii; eauto;
+    try(
+      specialize(H0 _ _ H1);
+      match goal with |- _ <= ?l + ?r => 
+        destruct (Nat.eq_dec x (l + r)); subst; omega || exfalso
+      end;
+      unfold IsSolution in *; destruct H1; ii;
+      specialize(H _ _ eq_refl); repeat match_destruct; congruence).
+    instantiate(m := AllMachine (S x) :: (fst map_step)).
+    destruct l; simpl in *; subst; ii.
+    invcs H1; specialize (H l r eq_refl).
+    destruct (AMSN (S l) r) eqn:?.
+    Apply AMSNSL; destruct Heqs; ii; right.
+    compute[map_step]; apply split_sum_In_fst; rewrite <- H3, H2 in *; apply in_map; ii.
+    Apply AMSNSR; ii.
+    rewrite H2 in *; ii.
+    destruct H2; ii.
+    rewrite H3 in *.
+    apply n0.
+    apply Exists_exists; econstructor; ii; eauto.
+    compute[map_step]; apply split_sum_In_snd; rewrite <- H4; apply in_map; ii.
+  Defined.
 
-Next Obligation.
-  compute[proj1_sig]; try omega.
-  destruct n; simpl in *.
-  pose proof (l n0 m0); ii.
-  destruct (Nat.eq_dec (n0 + m0) x); subst; try omega.
-  exfalso; specialize(H n0 m0 eq_refl); unfold HasSolution in *.
-  unfold SmallestSolution, HasSolution in *; ii.
-  destruct H1; match_destruct; ii; congruence.
-Defined.
-
-Next Obligation.
-  destruct l, n; simpl in *; subst; ii.
-  invcs H0; specialize(H l r eq_refl); match_destruct.
-  Apply AMSNSL; destruct H0; ii; rewrite H1 in *.
-  right; apply split_sum_In_fst; rewrite <- H2; apply in_map; ii.
-  Apply AMSNSR; ii.
-  rewrite H2 in *; ii.
-  destruct H2; ii; rewrite H2 in *.
-  apply X; apply Exists_exists; econstructor; ii; eauto.
-  apply split_sum_In_snd; rewrite <- H3; apply in_map; ii.
-Defined.
-Definition StepSmallestSolution n := exists l r, SmallestSolution l r /\ n = l + r.
-Next Obligation.
-  apply measure_wf; destruct SmallestSolutionExists as [? []].
-  match goal with |- well_founded ?P => replace P with (fun l r : nat => r < l <= (x + x0)) end.
-  apply Nat.gt_wf.
-  repeat ext; apply PE; unfold SmallestSolution in *; ii.
-  specialize(H3 n m H6); omega.
-  eapply H5; eauto.
-Defined.
-Program Definition UniversalSearch : { t | P t } := UniversalSearchAux 0 [AllMachine 0] _.
-Next Obligation.
-  omega.
-Defined.
-Next Obligation.
-  simpl in *.
-  destruct l, r; try omega.
-  unfold AMSN; simpl in *; tauto.
-Defined.
+  Program Definition UniversalSearch : { t | P t } := @UniversalSearchAux 0 [AllMachine 0] _ _.
+  Next Obligation.
+    simpl in *.
+    destruct l, r; try omega.
+    unfold AMSN; simpl in *; tauto.
+  Defined.
+  Solve All Obligations with program_simpl; omega.
+End UniversalSearch.
+Recursive Extraction UniversalSearch.
